Delimit modules and fixup notation

cava/Cava/Arrow/CavaNotation.v
@@ -43,7 +43,13 @@ Inductive NotationExpr: Kind -> Kind -> Type :=
 Definition instantiate {x y var} (e: NotationExpr x y) : kappa var x y :=
   match e with
   | ModuleExpr e => CallModule (module_instantiate_var e)
-  | FragmentExpr e => e var
+  | FragmentExpr e => RemoveContext (e var)
+  end.
+
+Definition notation_to_kappa {x y} (e: NotationExpr x y) : Kappa x y :=
+  match e with
+  | ModuleExpr e => module_body e
+  | FragmentExpr e => e
   end.
 
 Class instantiatable_expr (expr: Type) x y := {
@@ -67,24 +73,36 @@ Definition frag_to_expr {x y} (e: Kappa x y) := FragmentExpr e.
 
 Coercion kappa_to_expr: Module >-> NotationExpr.
 Coercion frag_to_expr: Kappa >-> NotationExpr.
+Coercion notation_to_kappa: NotationExpr >-> Kappa.
 
 Module KappaNotation.
 
-  Notation "<[ e ]>" := (
-    mkModule (fun var => e%kappa)
-   ) (at level 1, e custom expr at level 1).
+  Notation "<[ 'fun' name x .. y : ret => e ]>" := (
+    mkModule name (fun var =>
+      (Abs (fun x => .. (Abs (fun y => e)) ..)) : kappa var _ ret
+    %kappa)
+   ) (at level 1, name constr at level 1, x closed binder, e custom expr at level 99).
 
-  Notation "<{ e }>" := (
-    (fun var => e%kappa):Kappa _ _
-   ) (at level 1, e custom expr at level 1).
+  Notation "<[ \ x .. y => e ]>" := (
+    (fun var => (Abs (fun x => .. (Abs (fun y => e)) ..))%kappa): Kappa _ _
+   ) (at level 1, x closed binder, e custom expr at level 1).
+
+  Notation "<[ \ x .. y : ret => e ]>" := (
+    (fun var => (Abs (fun x => .. (Abs (fun y => e)) ..))%kappa): Kappa _ ret
+   ) (at level 1, x closed binder, e custom expr at level 1).
+
+  Notation "<[ e ]>" := (
+    (fun var => (e)%kappa): Kappa _ _
+   ) (at level 1, e custom expr at level 99).
+
+  (* Notation "<[ e ]>" := ( *)
+  (*   (fun var => e%kappa) : Kappa _ _ *)
+  (*  ) (at level 1, e custom expr at level 1). *)
+
+  (* Notation "\ x .. y => e" := (Abs (fun x => .. (Abs (fun y => e)) ..)) *)
+  (*   (in custom expr at level 200, x binder, right associativity) : kappa_scope. *)
 
   Notation "x ~> y" := (NotationExpr x y).
-
-  Notation Fragment x y := (Kappa x y).
-  Notation Module x y := (Module (Kappa x y)).
-
-  Notation "\ x .. y => e" := (Abs (fun x => .. (Abs (fun y => e)) ..))
-    (in custom expr at level 200, x binder, right associativity) : kappa_scope.
 
   Notation "x y" := (App x y) (in custom expr at level 3, left associativity) : kappa_scope.
 
@@ -97,138 +115,20 @@ Module KappaNotation.
   Notation "'letrec' x = a 'in' b" := (LetRec (fun x => a) (fun x => b))
     (in custom expr at level 1, x constr at level 4, b at level 7, a at level 1) : kappa_scope.
 
-  (* TODO(blaxill): can this be turned into a recursive pattern?
-  The binders not mentioned on the lhs (e.g. a_binder) prevent me from doing this
-  I think. Moving away from PHOAS would also work *)
+  (* destructuring *)
+  Notation "'let' '( x , .. , y ) : ty = a 'in' e" := (
+    Let (a : kappa _ Unit ty) (fun a_var => Comp1
+      (Abs (fun x => .. (Abs (fun y => e)) ..) )
+      (Var a_var : kappa _ Unit ty)
+    ) )
+    ( in custom expr at level 1, x closed binder, ty constr at level 7, e at level 7) : kappa_scope.
 
-  (* This function shouldn't be necessary but helps with type unification when
-  using the tuple destructuring notation *)
-  Definition proj1_tuple1 ty: CircuitPrimitive :=
-    match ty with
-    | Tuple l r => P1 (Fst l r)
-    | _ => P1 (Fst Unit Unit)
-    end.
-
-  Notation "'let' '( x , y ) = a 'in' b" := (
-    Let a (fun a_binder =>
-    Let (App (Primitive (P1 (Fst _ _))) (Var a_binder)) (fun x =>
-      Let (App (Primitive (P1 (Snd _ _))) (Var a_binder)) (fun y => b))))
-    ( in custom expr at level 1, x constr, y constr, b at level 7) : kappa_scope.
-
-  Notation "'let' '( x , y ) : ty = a 'in' b" := (
-    Let a (fun a_binder =>
-    Let (App (Primitive (proj1_tuple1 ty)) (Var a_binder)) (fun x =>
-      Let (App (Primitive (P1 (Snd _ _ ))) (Var a_binder)) (fun y => b))))
-    ( in custom expr at level 1, x constr, y constr, ty constr at level 7, b at level 7) : kappa_scope.
-
-  Notation "'let' '( x , y , z ) = a 'in' b" := (
-    Let a (fun a_binder =>
-    Let (App (Primitive (P1 (Fst _ _ ))) (Var a_binder)) (fun x =>
-      Let (App (Primitive (P1 (Snd _ _ ))) (Var a_binder)) (fun a_tl_binder =>
-        Let (App (Primitive (P1 (Fst _ _ ))) (Var a_tl_binder)) (fun y =>
-          Let (App (Primitive (P1 (Snd _ _ ))) (Var a_tl_binder)) (fun z =>
-          b))))))
-    ( in custom expr at level 1, x constr, y constr, z constr, b at level 7) : kappa_scope.
-  Notation "'let' '( x , y , z , w ) = a 'in' b" := (
-    Let a (fun a_binder =>
-    Let (App (Primitive (P1 (Fst _ _ ))) (Var a_binder)) (fun x =>
-      Let (App (Primitive (P1 (Snd _ _ ))) (Var a_binder)) (fun a_tl_binder =>
-        Let (App (Primitive (P1 (Fst _ _ ))) (Var a_tl_binder)) (fun y =>
-            Let (App (Primitive (P1 (Snd _ _ ))) (Var a_tl_binder)) (fun a_tl_tl_binder =>
-              Let (App (Primitive (P1 (Fst _ _ ))) (Var a_tl_tl_binder)) (fun z =>
-                Let (App (Primitive (P1 (Snd _ _ ))) (Var a_tl_tl_binder)) (fun w =>
-          b))))))))
-    ( in custom expr at level 1, x constr, y constr, z constr, w constr, b at level 7) : kappa_scope.
-  Notation "'let' '( x1 , x2 , x3 , x4 , x5 ) = a 'in' b" := (
-    Let a (fun binder1 =>
-    Let (App (Primitive (P1 (Fst _ _ ))) (Var binder1)) (fun x1 =>
-      Let (App (Primitive (P1 (Snd _ _ ))) (Var binder1)) (fun binder2 =>
-        Let (App (Primitive (P1 (Fst _ _ ))) (Var binder2)) (fun x2 =>
-            Let (App (Primitive (P1 (Snd _ _ ))) (Var binder2)) (fun binder3 =>
-              Let (App (Primitive (P1 (Fst _ _ ))) (Var binder3)) (fun x3 =>
-                Let (App (Primitive (P1 (Snd _ _ ))) (Var binder3)) (fun binder4 =>
-                  Let (App (Primitive (P1 (Fst _ _ ))) (Var binder4)) (fun x4 =>
-                    Let (App (Primitive (P1 (Snd _ _ ))) (Var binder4)) (fun x5 =>
-          b))))))))))
-    ( in custom expr at level 1
-    , x1 constr, x2 constr, x3 constr, x4 constr, x5 constr
-    , b at level 7) : kappa_scope.
-  Notation "'let' '( x1 , x2 , x3 , x4 , x5 , x6 ) = a 'in' b" := (
-    Let a (fun binder1 =>
-    Let (App (Primitive (P1 (Fst _ _ ))) (Var binder1)) (fun x1 =>
-      Let (App (Primitive (P1 (Snd _ _ ))) (Var binder1)) (fun binder2 =>
-        Let (App (Primitive (P1 (Fst _ _ ))) (Var binder2)) (fun x2 =>
-            Let (App (Primitive (P1 (Snd _ _ ))) (Var binder2)) (fun binder3 =>
-              Let (App (Primitive (P1 (Fst _ _ ))) (Var binder3)) (fun x3 =>
-                Let (App (Primitive (P1 (Snd _ _ ))) (Var binder3)) (fun binder4 =>
-                  Let (App (Primitive (P1 (Fst _ _ ))) (Var binder4)) (fun x4 =>
-                    Let (App (Primitive (P1 (Snd _ _ ))) (Var binder4)) (fun binder5 =>
-                      Let (App (Primitive (P1 (Fst _ _ ))) (Var binder5)) (fun x5 =>
-                        Let (App (Primitive (P1 (Snd _ _ ))) (Var binder5)) (fun x6 =>
-          b))))))))))))
-    ( in custom expr at level 1
-    , x1 constr, x2 constr, x3 constr, x4 constr, x5 constr, x6 constr
-    , b at level 7) : kappa_scope.
-  Notation "'let' '( x1 , x2 , x3 , x4 , x5 , x6 , x7 ) = a 'in' b" := (
-    Let a (fun binder1 =>
-    Let (App (Primitive (P1 (Fst _ _ ))) (Var binder1)) (fun x1 =>
-      Let (App (Primitive (P1 (Snd _ _ ))) (Var binder1)) (fun binder2 =>
-        Let (App (Primitive (P1 (Fst _ _ ))) (Var binder2)) (fun x2 =>
-            Let (App (Primitive (P1 (Snd _ _ ))) (Var binder2)) (fun binder3 =>
-              Let (App (Primitive (P1 (Fst _ _ ))) (Var binder3)) (fun x3 =>
-                Let (App (Primitive (P1 (Snd _ _ ))) (Var binder3)) (fun binder4 =>
-                  Let (App (Primitive (P1 (Fst _ _ ))) (Var binder4)) (fun x4 =>
-                    Let (App (Primitive (P1 (Snd _ _ ))) (Var binder4)) (fun binder5 =>
-                      Let (App (Primitive (P1 (Fst _ _ ))) (Var binder5)) (fun x5 =>
-                        Let (App (Primitive (P1 (Snd _ _ ))) (Var binder5)) (fun binder6 =>
-                            Let (App (Primitive (P1 (Fst _ _ ))) (Var binder6)) (fun x6 =>
-                              Let (App (Primitive (P1 (Snd _ _ ))) (Var binder6)) (fun x7 =>
-          b))))))))))))))
-    ( in custom expr at level 1
-    , x1 constr, x2 constr, x3 constr, x4 constr, x5 constr, x6 constr, x7 constr
-    , b at level 7) : kappa_scope.
-
-  Notation "'let' '( x1 , x2 , x3 , x4 , x5 , x6 , x7 ) : ty = a 'in' b" := (
-    Let a (fun binder1 =>
-    Let (App (Primitive (proj1_tuple1 ty)) (Var binder1)) (fun x1 =>
-      Let (App (Primitive (P1 (Snd _ _ ))) (Var binder1)) (fun binder2 =>
-        Let (App (Primitive (P1 (Fst _ _ ))) (Var binder2)) (fun x2 =>
-            Let (App (Primitive (P1 (Snd _ _ ))) (Var binder2)) (fun binder3 =>
-              Let (App (Primitive (P1 (Fst _ _ ))) (Var binder3)) (fun x3 =>
-                Let (App (Primitive (P1 (Snd _ _ ))) (Var binder3)) (fun binder4 =>
-                  Let (App (Primitive (P1 (Fst _ _ ))) (Var binder4)) (fun x4 =>
-                    Let (App (Primitive (P1 (Snd _ _ ))) (Var binder4)) (fun binder5 =>
-                      Let (App (Primitive (P1 (Fst _ _ ))) (Var binder5)) (fun x5 =>
-                        Let (App (Primitive (P1 (Snd _ _ ))) (Var binder5)) (fun binder6 =>
-                            Let (App (Primitive (P1 (Fst _ _ ))) (Var binder6)) (fun x6 =>
-                              Let (App (Primitive (P1 (Snd _ _ ))) (Var binder6)) (fun x7 =>
-          b))))))))))))))
-    ( in custom expr at level 1
-    , x1 constr, x2 constr, x3 constr, x4 constr, x5 constr, x6 constr, x7 constr
-    , ty constr at level 7
-    , b at level 7) : kappa_scope.
-
-  Notation "'let' '( x1 , x2 , x3 , x4 , x5 , x6 , x7 , x8 ) : ty = a 'in' b" := (
-    Let a (fun binder1 =>
-    Let (App (Primitive (proj1_tuple1 ty)) (Var binder1)) (fun x1 =>
-      Let (App (Primitive (P1 (Snd _ _ ))) (Var binder1)) (fun binder2 =>
-        Let (App (Primitive (P1 (Fst _ _ ))) (Var binder2)) (fun x2 =>
-            Let (App (Primitive (P1 (Snd _ _ ))) (Var binder2)) (fun binder3 =>
-              Let (App (Primitive (P1 (Fst _ _ ))) (Var binder3)) (fun x3 =>
-                Let (App (Primitive (P1 (Snd _ _ ))) (Var binder3)) (fun binder4 =>
-                  Let (App (Primitive (P1 (Fst _ _ ))) (Var binder4)) (fun x4 =>
-                    Let (App (Primitive (P1 (Snd _ _ ))) (Var binder4)) (fun binder5 =>
-                      Let (App (Primitive (P1 (Fst _ _ ))) (Var binder5)) (fun x5 =>
-                        Let (App (Primitive (P1 (Snd _ _ ))) (Var binder5)) (fun binder6 =>
-                            Let (App (Primitive (P1 (Fst _ _ ))) (Var binder6)) (fun x6 =>
-                              Let (App (Primitive (P1 (Snd _ _ ))) (Var binder6)) (fun binder7 =>
-                                  Let (App (Primitive (P1 (Fst _ _ ))) (Var binder7)) (fun x7 =>
-                                    Let (App (Primitive (P1 (Snd _ _ ))) (Var binder7)) (fun x8 =>
-          b))))))))))))))))
-    ( in custom expr at level 1
-    , x1 constr, x2 constr, x3 constr, x4 constr, x5 constr, x6 constr, x7 constr, x8 constr
-    , ty constr at level 7
-    , b at level 7) : kappa_scope.
+  Notation "'let' '( x , .. , y ) = a 'in' e" := (
+    Let a (fun a_var => Comp1
+      (Abs (fun x => .. (Abs (fun y => e)) ..) )
+      (Var a_var )
+    ) )
+    ( in custom expr at level 1, x closed binder, e at level 7) : kappa_scope.
 
   (* Escaping *)
 
@@ -336,47 +236,50 @@ Section regression_examples.
   Import KappaNotation.
   Local Open Scope kappa_scope.
 
-  Program Definition ex0_constant: Module << Vector Bit 10, Unit >> (Vector Bit 8)
-    := <[ \x => x [: 7 : 0 ] ]>.
+  Definition ex0_constant
+    := <[ fun "ex0_constant" ( x : _ (Vector Bit 8) ) : Vector Bit 8 => x [: 7 : 0 ] ]>.
 
-  Definition ex1_constant: Fragment << Bit, Unit >> Bit := <{ \x => true' }>.
-  Definition ex2_parameterized (n: nat): Fragment << Bit, Unit >> Bit :=
+  Definition ex1_constant: Kappa << Bit, Unit >> Bit := <[ \ x => true' ]> .
+
+  Definition ex2_parameterized (n: nat): Kappa << Bit, Unit >> Bit :=
   match n with
-  | O => <{ \ x => true' }>
-  | S n => <{ \ x => xor x x }>
+  | O => <[\x => true' ]>
+  | S n => <[\x => xor x x ]>
   end.
 
-  Definition ex3_to_vec: Module << Bit, Unit >> (Vector Bit 1) :=
+  Definition ex3_to_vec: Kappa << Bit, Unit >> (Vector Bit 1) :=
   <[ \ x => x :: [] ]>.
-  Definition ex4_index_vec:  Module << Vector Bit 10, Unit >> Bit :=
+  Definition ex4_index_vec:  Kappa << Vector Bit 10, Unit >> Bit :=
   <[ \ x => index x (# 1) ]>.
-  Definition ex5_index_vec2:  Module << Vector Bit 10, Unit >> Bit :=
+  Definition ex5_index_vec2:  Kappa << Vector Bit 10, Unit >> Bit :=
   <[ \ x => x [# 1] ]>.
-  Definition ex6_concat:  Module << Vector Bit 2, Bit, Unit >> (Vector Bit 3) :=
+  Definition ex6_concat:  Kappa << Vector Bit 2, Bit, Unit >> (Vector Bit 3) :=
   <[ \ x v => snoc x v ]>.
-  Definition ex7_xor:  Module << Bit, Bit, Unit >> Bit :=
-  <[ \ x y => xor x y ]>.
-  Definition ex7_tupled_destruct:  Module << << Bit, Bit>>, Unit>> Bit :=
+
+  Definition ex7_xor :=
+    <[fun "ex7_xor" (x : _ Bit) (y : _ Bit) : Bit => xor x y ]>.
+
+  Definition ex7_tupled_destruct:  Kappa << << Bit, Bit>>, Unit>> Bit :=
   <[ \ xy =>
     let '(x,y) : <<Bit,Bit>> = xy in
     y ]>.
-  Definition ex8_multiindex:  Module << Vector (Vector Bit 5) 10, Unit >> Bit :=
+  Definition ex8_multiindex:  Kappa << Vector (Vector Bit 5) 10, Unit >> Bit :=
   <[ \ x => x[#0][#1] ]>.
-  Definition ex9_mkvec:  Module << Bit, Unit >> (Vector Bit 2) :=
+  Definition ex9_mkvec:  Kappa << Bit, Unit >> (Vector Bit 2) :=
   <[ \x => true' :: false' :: [] ]>.
-  Definition ex10:  Module << Vector Bit 10, Vector Bit 10, Unit >> (Vector Bit 11) :=
+  Definition ex10:  Kappa << Vector Bit 10, Vector Bit 10, Unit >> (Vector Bit 11) :=
   <[ \ x y => x + y ]>.
-  Definition ex11:  Module << Vector Bit 10, Vector Bit 10, Unit >> (Vector Bit 10) :=
+  Definition ex11:  Kappa << Vector Bit 10, Vector Bit 10, Unit >> (Vector Bit 10) :=
   <[ \ x y => x +% y ]>.
-  Definition ex13:  Module << Vector Bit 10, Unit >> Bit :=
+  Definition ex13:  Kappa << Vector Bit 10, Unit >> Bit :=
   <[ \ x => (xor x[#0] x[#1] :: false' :: []) [#0] ]>.
-  Definition ex14:  Module << Vector Bit 10, Vector Bit 4, Unit >> Bit :=
+  Definition ex14:  Kappa << Vector Bit 10, Vector Bit 4, Unit >> Bit :=
   <[ \ x i => x [ i ] ]>.
-  Definition ex15_rec_xor:  Module << Bit, Unit >> Bit :=
+  Definition ex15_rec_xor:  Kappa << Bit, Unit >> Bit :=
   <[ \ x => letrec s = delay (xor x s) in s ]>.
-  Definition ex16_triple:  Module << <<Bit, Bit, Bit>>, Unit >> Bit :=
-  <[ \ triple => let '(x, y, z) = triple in x ]>.
-  Definition ex17_constant_via_list: Module << Unit >> (Vector (Vector Bit 4) 3) := <[  { 1, 2, 3 } ]>.
+  Definition ex16_triple:  Kappa << <<Bit, Bit, Bit>>, Unit >> Bit :=
+  <[ \ triple => let '(x, y, z) : <<Bit,Bit,Bit>> = triple in x ]>.
+  Definition ex17_constant_via_list: Kappa << Unit >> (Vector (Vector Bit 4) 3) := <[ { 1, 2, 3 } ]>.
 
   Fixpoint copy_object_pow2 o (n:nat): Kind :=
   match n with
@@ -384,30 +287,30 @@ Section regression_examples.
   | S n => Tuple (copy_object_pow2 o n) (copy_object_pow2 o n)
   end.
 
-  Program Fixpoint tree
+  Fixpoint tree
     (A: Kind)
     (n: nat)
     (f: << A, A, Unit >> ~> A)
     {struct n}
-    : Fragment << copy_object_pow2 A n, Unit >> A :=
+    : Kappa << copy_object_pow2 A n, Unit >> A :=
   match n with
   | O =>
-    <{ \ x => x }>
+    <[ \ x => x ]>
   | S n' =>
-    <{\ x =>
+    <[\ x =>
         let a = !(tree n' f) (fst x) in
         let b = !(tree n' f) (snd x) in
         !f a b
-    }>
+    ]>
   end.
 
-  Program Definition adder_tree
+  Definition adder_tree
     (bitsize n: nat)
-    : Module <<copy_object_pow2 (Vector Bit bitsize) n, Unit>> (Vector Bit bitsize) :=
-    <[ !(tree n <{\x y => x +% y}> ) ]>.
+    : Kappa <<copy_object_pow2 (Vector Bit bitsize) n, Unit>> (Vector Bit bitsize) :=
+    <[ !(tree n <[\x y => x +% y]> ) ]>.
 
   Definition xilinxFullAdder
-    : Module << Bit, << Bit, Bit >>, Unit>> (Tuple Bit Bit) :=
+    : Kappa << Bit, << Bit, Bit >>, Unit>> (Tuple Bit Bit) :=
     <[ \ cin ab =>
       let a = fst ab in
       let b = snd ab in
@@ -418,28 +321,28 @@ Section regression_examples.
     ]>.
 
   Fixpoint reshape {n m A}
-    : Fragment << Vector A (n * m), Unit >> << Vector (Vector A m) n >> :=
+    : Kappa << Vector A (n * m), Unit >> << Vector (Vector A m) n >> :=
   match n with
-  | 0 => <{\_ => [] }>
+  | 0 => <[\_ => [] ]>
   | S n' =>
-    <{ \vec =>
-      let '(x, xs) = split_at m vec in
+    <[ \vec =>
+      let '(x, xs) : <<Vector A _, Vector A _>> = split_at m vec in
       x :: !(@reshape n' m A) xs
-      }>
+      ]>
   end.
 
   Definition dummy {T}
-    : Module << Bit, T, T, Unit >> <<T>> :=
+    : Kappa << Bit, T, T, Unit >> <<T>> :=
     <[\_ x _ => x]>.
   Notation T:=(Bit )(only parsing).
   Notation "'if' i 'then' t 'else' e" :=
-    (App (App (App (instantiate dummy) i) t) e)
+    (App (App (App (instantiate (embed_expr dummy)) i) t) e)
     (in custom expr at level 5, left associativity) : kappa_scope.
 
-  Definition exfailed: Module << <<T,T>>,<<T,T>>, Unit >> <<T,T>> :=
+  Definition exfailed: Kappa << <<T,T>>,<<T,T>>, Unit >> <<T,T>> :=
     <[\s1 s2 =>
     let '(a,b) : <<_,T>> =  s1 in
-    let '(aa,bb) : <<_,_>> = s2 in
+    let '(aa,bb) : <<_,T>> = s2 in
     if a then (a,b) else s1
     ]>.
 
